BitFields: porting the remaining lemmas to the bitfields
Signed-off-by: Reto Achermann <achreto@cs.ubc.ca>

src/BitFields/MachineWords.i.dfy
@@ -1,3 +1,29 @@
+/*
+ * MIT License
+ *
+ * Copyright (c) 2022 Reto Achermann, The University of British Columbia
+ *
+ * Permission is hereby granted, free of charge, to any person obtaining a copy
+ * of this software and associated documentation files (the "Software"), to deal
+ * in the Software without restriction, including without limitation the rights
+ * to use, copy, modify, merge, publish, distribute, sublicense, and/or sell
+ * copies of the Software, and to permit persons to whom the Software is
+ * furnished to do so, subject to the following conditions:
+ *
+ * The above copyright notice and this permission notice shall be included in all
+ * copies or substantial portions of the Software.
+ *
+ * THE SOFTWARE IS PROVIDED "AS IS", WITHOUT WARRANTY OF ANY KIND, EXPRESS OR
+ * IMPLIED, INCLUDING BUT NOT LIMITED TO THE WARRANTIES OF MERCHANTABILITY,
+ * FITNESS FOR A PARTICULAR PURPOSE AND NONINFRINGEMENT. IN NO EVENT SHALL THE
+ * AUTHORS OR COPYRIGHT HOLDERS BE LIABLE FOR ANY CLAIM, DAMAGES OR OTHER
+ * LIABILITY, WHETHER IN AN ACTION OF CONTRACT, TORT OR OTHERWISE, ARISING FROM,
+ * OUT OF OR IN CONNECTION WITH THE SOFTWARE OR THE USE OR OTHER DEALINGS IN THE
+ * SOFTWARE.
+ *
+ * SPDX-License-Identifier: MIT
+ */
+
 include "Spec/MachineTypes.s.dfy"
 include "BitFields.i.dfy"
 
@@ -43,6 +69,51 @@ module MachineWords {
     function UInt8ToInt(a: uint8) : int { a as int}
     function UInt8ToNat(a: uint8) : int { a as nat}
 
+    ///////////////////////////////////////////////////////////////////////////////////////////////
+    // Helper Functions
+    ///////////////////////////////////////////////////////////////////////////////////////////////
+
+    /// a predicate for the inrange condition of the bits
+    /// intended to be used in foralls.
+    predicate InRange(i:uint64, n:uint64) {
+        0 <= i && i < n
+    }
+
+
+    ///////////////////////////////////////////////////////////////////////////////////////////////
+    // From/To Seq<bool>
+    ///////////////////////////////////////////////////////////////////////////////////////////////
+
+    function {:opaque} BitwiseToSeqBool(b: uint64) : (r: seq<bool>)
+        ensures |r| == B.WORD_SIZE as nat
+        ensures forall i | InRange(i, B.WORD_SIZE) :: r[i] == BitwiseGetBit(b, i)
+    {
+        reveal_BitwiseGetBit();
+        B.BitsToSeqBool(B.WordToBits(b))
+    }
+
+    function {:opaque} SeqBoolToBitwise(b: seq<bool>) : (r: uint64)
+        requires |b| == B.WORD_SIZE as nat
+        ensures forall i | InRange(i, |b| as uint64) :: b[i] == BitwiseGetBit(r, i)
+    {
+        reveal_BitwiseGetBit(); B.reveal_BitsToWord();
+        B.lemma_BitsToWordWordToBits(B.SeqBoolToBits(b));
+        B.BitsToWord(B.SeqBoolToBits(b))
+    }
+
+    lemma lemma_SeqToBitsToSeq(b: seq<bool>)
+        requires |b| == B.WORD_SIZE as nat
+        ensures BitwiseToSeqBool(SeqBoolToBitwise(b)) == b
+    {
+    }
+
+    lemma lemma_BitsToSeqToBits(b: uint64)
+        ensures SeqBoolToBitwise(BitwiseToSeqBool(b)) == b
+    {
+        var b' := SeqBoolToBitwise(BitwiseToSeqBool(b));
+        assert forall i | InRange(i, B.WORD_SIZE) :: (BitwiseGetBit(b', i) == BitwiseGetBit(b, i));
+        lemma_BitwiseEq(b, b');
+    }
 
     ///////////////////////////////////////////////////////////////////////////////////////////////
     // Constructor Functions
@@ -61,6 +132,12 @@ module MachineWords {
 
     function method BitwiseZeros() : uint64 {
         0x0
+    }
+
+    function method {:opaque} BitwiseMask(i: uint64) : uint64
+        requires i <= B.WORD_SIZE
+    {
+        B.BitsToWord(B.BitMask(i))
     }
 
     ///////////////////////////////////////////////////////////////////////////////////////////////
@@ -113,19 +190,8 @@ module MachineWords {
         requires i < B.WORD_SIZE
         ensures BitwiseGetBit(r, i) != BitwiseGetBit(a, i)
     {
-        var bv_a := B.WordToBits(a);
-        var bv_r := B.BitToggleBit(bv_a, i);
-        var r    := B.BitsToWord(bv_r);
-
-        assert B.BitIsSet(bv_a, i) != B.BitIsSet(bv_r, i);
-
-        assert BitwiseGetBit(r, i) != BitwiseGetBit(a, i) by {
-            reveal_BitwiseGetBit();
-            B.lemma_BitsToWordWordToBits(bv_a);
-            B.lemma_BitsToWordWordToBits(bv_r);
-        }
-
-        r
+        if BitwiseGetBit(a, i) then BitwiseClearBit(a, i)
+        else BitwiseSetBit(a, i)
     }
 
     ///////////////////////////////////////////////////////////////////////////////////////////////
@@ -239,13 +305,14 @@ module MachineWords {
     }
 
     lemma lemma_BitwiseAndZero(a: uint64)
-        ensures BitwiseAnd(a, 0) == 0
+        ensures BitwiseAnd(a, BitwiseZeros()) == BitwiseZeros()
     {
         var bv_a := B.WordToBits(a);
         B.reveal_WordToBits();
         reveal_BitwiseAnd();
         B.lemma_BitAndZero(bv_a);
         B.reveal_BitsToWord();
+        B.reveal_BitZeros();
     }
 
     lemma lemma_BitwiseAndOnes(a: uint64)
@@ -262,6 +329,13 @@ module MachineWords {
         B.lemma_BitAndOnes(bv_a);
         B.lemma_WordToBitsBitsToWord(a);
         B.reveal_WordToBits();
+    }
+
+    lemma lemma_BitwiseAndOnesEq(a: uint64, b: uint64)
+        ensures (a == b) <==> (BitwiseAnd(a, BitwiseOnes()) == BitwiseAnd(b, BitwiseOnes()))
+    {
+        lemma_BitwiseAndOnes(a);
+        lemma_BitwiseAndOnes(b);
     }
 
     lemma lemma_BitwiseAndComm(a: uint64, b: uint64)
@@ -310,6 +384,7 @@ module MachineWords {
         B.lemma_BitAndCompSelf(bv_a);
         B.lemma_BitsToWordWordToBits(B.BitComp(bv_a));
         B.reveal_BitsToWord();
+        B.reveal_BitZeros();
     }
 
     lemma lemma_BitwiseAndNotSelf(a: uint64)
@@ -323,11 +398,13 @@ module MachineWords {
         B.lemma_BitAndNotSelf(bv_a);
         B.lemma_BitsToWordWordToBits(B.BitNot(bv_a));
         B.reveal_BitsToWord();
+        B.reveal_BitZeros();
     }
 
     lemma lemma_BitwiseAndBitDist(a: uint64, b: uint64, i: uint64)
         requires i < B.WORD_SIZE
-        ensures (BitwiseAnd(BitwiseAnd(a, BitwiseBit(i)), BitwiseAnd(b, BitwiseBit(i))) == 0)  ==  ((BitwiseAnd(a, BitwiseBit(i)) == 0) || (BitwiseAnd(b, BitwiseBit(i)) == 0))
+        ensures (BitwiseAnd(BitwiseAnd(a, BitwiseBit(i)), BitwiseAnd(b, BitwiseBit(i))) == 0)
+                    ==  ((BitwiseAnd(a, BitwiseBit(i)) == 0) || (BitwiseAnd(b, BitwiseBit(i)) == 0))
     {
         var bv_a := B.WordToBits(a);
         var bv_b := B.WordToBits(b);
@@ -336,6 +413,7 @@ module MachineWords {
         B.lemma_BitsToWordWordToBits(B.Bit(i));
         B.lemma_BitsToWordWordToBits(B.BitAnd(bv_a, B.Bit(i))); B.lemma_BitsToWordWordToBits(B.BitAnd(bv_b, B.Bit(i)));
         B.lemma_BitAndBitDist(bv_a, bv_b, i);
+        B.reveal_BitZeros();
     }
 
     lemma lemma_BitwiseAndIsIntersection(a: uint64, b: uint64, i : uint64)
@@ -370,7 +448,7 @@ module MachineWords {
         var bv_a := B.WordToBits(a);
 
         reveal_BitwiseOr();
-        B.reveal_WordToBits();
+        B.reveal_WordToBits(); B.reveal_BitZeros();
         B.lemma_BitOrZero(bv_a);
         B.lemma_WordToBitsBitsToWord(a);
     }
@@ -434,8 +512,7 @@ module MachineWords {
         var bv_b := B.WordToBits(b);
 
         reveal_BitwiseOr();
-        B.reveal_BitsToWord();
-        B.reveal_WordToBits();
+        B.reveal_BitsToWord(); B.reveal_WordToBits(); B.reveal_BitZeros();
         B.lemma_BitOrZeroImpliesArgs(bv_a, bv_b);
     }
 
@@ -463,7 +540,7 @@ module MachineWords {
         var bv_a := B.WordToBits(a);
 
         reveal_BitwiseXor();
-        B.reveal_BitsToWord();
+        B.reveal_BitsToWord(); B.reveal_BitZeros();
         B.lemma_BitXorSelf(bv_a);
     }
 
@@ -473,7 +550,7 @@ module MachineWords {
         var bv_a := B.WordToBits(a);
 
         reveal_BitwiseXor();
-        B.reveal_WordToBits();
+        B.reveal_WordToBits(); B.reveal_BitZeros();
         B.lemma_BitXorZero(bv_a);
         B.lemma_WordToBitsBitsToWord(a);
     }
@@ -526,10 +603,12 @@ module MachineWords {
         reveal_BitwiseXor();
         B.lemma_WordToBitsBitsToWord(a);
         B.lemma_WordToBitsBitsToWord(b);
-        assert B.BitXor(bv_a, bv_b) == 0 by {
+        B.reveal_BitZeros();
+        assert B.BitXor(bv_a, bv_b) == B.BitZeros() by {
             B.reveal_BitsToWord();
             B.reveal_WordToBits();
         }
+
         B.lemma_BitXorZeroImpliesArgs(bv_a, bv_b);
     }
 
@@ -590,6 +669,17 @@ module MachineWords {
         B.lemma_BitsToWordWordToBits(B.BitNot(bv_a));
     }
 
+
+    lemma lemma_BitwiseNotOnes()
+        ensures BitwiseNot(BitwiseOnes()) == BitwiseZeros();
+        ensures BitwiseNot(BitwiseZeros()) == BitwiseOnes();
+    {
+        reveal_BitwiseNot();
+        B.lemma_BitNotOnes();
+        B.reveal_BitNot(); B.reveal_BitZeros(); B.reveal_BitOnes();
+        B.reveal_WordToBits(); B.reveal_BitsToWord();
+    }
+
     ///////////////////////////////////////////////////////////////////////////////////////////////
     // Shifts
     ///////////////////////////////////////////////////////////////////////////////////////////////
@@ -609,6 +699,7 @@ module MachineWords {
         reveal_BitwiseBit();
         B.reveal_BitsToWord();
         B.lemma_BitNotZero(i);
+        B.reveal_BitZeros();
     }
 
     lemma lemma_BitBitIsSet(i: uint64)
@@ -645,6 +736,7 @@ module MachineWords {
         B.reveal_BitsToWord();
         B.lemma_BitsToWordWordToBits(B.Bit(i));
         B.lemma_BitsToWordWordToBits(B.Bit(j));
+        B.reveal_BitZeros();
     }
 
     lemma lemma_BitwiseOnesBitIsSet(i: uint64)
@@ -669,9 +761,105 @@ module MachineWords {
         B.lemma_BitZerosNotBitIsSet(i);
     }
 
+    lemma lemma_BitwiseMaskIsOnes()
+        ensures BitwiseMask(64) == BitwiseOnes()
+    {
+        reveal_BitwiseMask();
+        B.reveal_BitMask();
+        B.reveal_BitsToWord(); B.reveal_WordToBits();
+        B.reveal_BitOnes();
+    }
+
+    lemma lemma_BitwiseMaskIsZeros()
+        ensures BitwiseMask(0) == BitwiseZeros()
+    {
+        reveal_BitwiseMask();
+        B.lemma_BitMaskIsZeros();
+        B.reveal_BitsToWord(); B.reveal_WordToBits();
+        B.reveal_BitZeros();
+    }
+
+    lemma lemma_BitwiseMaskExtendBitOr(i: uint64)
+        requires i < B.WORD_SIZE
+        ensures BitwiseMask(i+1) == BitwiseOr(BitwiseMask(i), BitwiseBit(i))
+    {
+        reveal_BitwiseMask(); reveal_BitwiseOr(); reveal_BitwiseBit();
+        B.lemma_BitsToWordWordToBits(B.BitMask(i));
+        B.lemma_BitsToWordWordToBits(B.Bit(i));
+        B.lemma_BitMaskExtendBitOr(i);
+    }
+
+    lemma lemma_BitwiseMaskExtendBitOrLess(i: uint64)
+        requires 0 < i <= B.WORD_SIZE
+        ensures BitwiseMask(i) == BitwiseOr(BitwiseMask(i-1), BitwiseBit(i-1))
+    {
+        reveal_BitwiseMask(); reveal_BitwiseOr(); reveal_BitwiseBit();
+        B.lemma_BitsToWordWordToBits(B.BitMask(i-1));
+        B.lemma_BitsToWordWordToBits(B.Bit(i-1));
+        B.lemma_BitMaskExtendBitOrLess(i);
+    }
+
+    lemma lemma_BitwiseMaskExtendBitSet(i: uint64)
+        requires i < B.WORD_SIZE
+        ensures BitwiseMask(i+1) == BitwiseSetBit(BitwiseMask(i), i)
+    {
+        reveal_BitwiseSetBit(); reveal_BitwiseMask();
+        B.lemma_BitsToWordWordToBits(B.BitMask(i));
+        B.lemma_BitMaskExtendBitSet(i);
+    }
+
+    lemma lemma_BitwiseMaskExtendBitSetLess(i: uint64)
+        requires 0 < i <= B.WORD_SIZE
+        ensures BitwiseMask(i) == BitwiseSetBit(BitwiseMask(i-1), i-1)
+    {
+        reveal_BitwiseSetBit(); reveal_BitwiseMask();
+        B.lemma_BitsToWordWordToBits(B.BitMask(i-1));
+        B.lemma_BitMaskExtendBitSetLess(i);
+    }
+
     ///////////////////////////////////////////////////////////////////////////////////////////////
     // Setting Individual Bits
     ///////////////////////////////////////////////////////////////////////////////////////////////
+
+    lemma lemma_BitwiseForallImpliesBitForall(a: uint64, b: uint64)
+        requires (forall j | InRange(j, B.WORD_SIZE) :: (BitwiseGetBit(a, j) == BitwiseGetBit(b, j)))
+        ensures  (forall j | B.InRange(j, B.WORD_SIZE) :: (B.BitIsSet(B.WordToBits(a), j) == B.BitIsSet(B.WordToBits(b), j)))
+    {
+        forall j | B.InRange(j, B.WORD_SIZE)
+        ensures (B.BitIsSet(B.WordToBits(a), j) == B.BitIsSet(B.WordToBits(b), j))
+        {
+            assert B.InRange(j, B.WORD_SIZE);
+            assert InRange(j, B.WORD_SIZE);
+            reveal_BitwiseGetBit();
+            assert BitwiseGetBit(a, j)  == B.BitIsSet(B.WordToBits(a), j);
+            assert BitwiseGetBit(b, j)  == B.BitIsSet(B.WordToBits(b), j);
+        }
+    }
+
+    lemma lemma_BitwiseAllBitsEqualBVEq(a: uint64, b: uint64)
+        requires (forall j | InRange(j, B.WORD_SIZE) :: (BitwiseGetBit(a, j) == BitwiseGetBit(b, j)))
+        ensures a == b
+    {
+        var bv_a := B.WordToBits(a);
+        var bv_b := B.WordToBits(b);
+
+        lemma_BitwiseForallImpliesBitForall(a, b);
+        B.lemma_AllBitsEqualBVEq(bv_a, bv_b);
+        B.lemma_BitsToWordEq(bv_a, bv_b);
+        B.lemma_WordToBitsBitsToWord(a);
+        B.lemma_WordToBitsBitsToWord(b);
+    }
+
+    lemma lemma_BitwiseEq(a: uint64, b: uint64)
+        ensures (a == b) == (forall i |  InRange(i, B.WORD_SIZE):: (BitwiseGetBit(a, i) == BitwiseGetBit(b, i)))
+    {
+        if (forall i |  InRange(i, B.WORD_SIZE):: (BitwiseGetBit(a, i) == BitwiseGetBit(b, i))) {
+            lemma_BitwiseAllBitsEqualBVEq(a, b);
+        } else {
+        }
+
+    }
+
 
     lemma lemma_BitwiseSetSelf(a: uint64, i: uint64)
         requires i < B.WORD_SIZE
@@ -709,6 +897,50 @@ module MachineWords {
         reveal_BitwiseGetBit(); reveal_BitwiseClearBit();
         B.lemma_BitsToWordWordToBits(B.BitClearBit(bv_a, i));
         B.lemma_BitClearOther(bv_a, i, j);
+    }
+
+    lemma lemma_BitwiseSetNotChangeOthers(a: uint64, i: uint64)
+        requires i < B.WORD_SIZE
+        ensures forall j | InRange(j, B.WORD_SIZE) && i != j :: BitwiseGetBit(a, j) == BitwiseGetBit(BitwiseSetBit(a, i), j)
+    {
+        var bv_a := B.WordToBits(a);
+        B.lemma_BitSetNotChangeOthers(bv_a, i);
+
+        forall j | InRange(j, B.WORD_SIZE) && i != j
+        ensures BitwiseGetBit(a, j) == BitwiseGetBit(BitwiseSetBit(a, i), j)
+        {
+            reveal_BitwiseGetBit(); reveal_BitwiseSetBit();
+            B.lemma_BitsToWordWordToBits(B.BitSetBit(bv_a, i));
+        }
+    }
+
+    lemma lemma_BitwiseClearNotChangeOthers(a: uint64, i: uint64)
+        requires i < B.WORD_SIZE
+        ensures forall j | InRange(j, B.WORD_SIZE) && i != j :: BitwiseGetBit(a, j) == BitwiseGetBit(BitwiseClearBit(a, i), j)
+    {
+        var bv_a := B.WordToBits(a);
+        B.lemma_BitClearNotChangeOthers(bv_a, i);
+
+        forall j | InRange(j, B.WORD_SIZE) && i != j
+        ensures BitwiseGetBit(a, j) == BitwiseGetBit(BitwiseClearBit(a, i), j)
+        {
+            reveal_BitwiseGetBit(); reveal_BitwiseClearBit();
+            B.lemma_BitsToWordWordToBits(B.BitClearBit(bv_a, i));
+        }
+    }
+
+    lemma lemma_BitwiseToggleNotChangeOthers(a: uint64, i: uint64)
+        requires i < B.WORD_SIZE
+        ensures forall j | InRange(j, B.WORD_SIZE) && i != j :: BitwiseGetBit(a, j) == BitwiseGetBit(BitwiseToggleBit(a, i), j)
+    {
+        reveal_BitwiseToggleBit();
+        if BitwiseGetBit(a, i) {
+            assert BitwiseToggleBit(a, i) == BitwiseClearBit(a, i);
+            lemma_BitwiseClearNotChangeOthers(a, i);
+        } else {
+            assert BitwiseToggleBit(a, i) == BitwiseSetBit(a, i);
+            lemma_BitwiseSetNotChangeOthers(a, i);
+        }
     }
 
     ///////////////////////////////////////////////////////////////////////////////////////////////
